extending bblock_simu_test with rewriting

mppa_k1c/abstractbb/Impure/ocaml/ImpHConsOracles.mli
@@ -1,4 +1,5 @@
 open ImpPrelude
+open HConsingDefs
 
-val make_dict : 'a1 Dict.hash_params -> ('a1, 'a2) Dict.t
-val xhCons: (('a -> 'a -> bool) * ('a pre_hashV -> 'a hashV)) -> 'a hashConsing
+val make_dict : 'a Dict.hash_params -> ('a, 'b) Dict.t
+val xhCons: 'a hashH -> 'a hashConsing
