mppa_k1c/abstractbb/SeqSimuTheory.v
@@ -1,0 +1,428 @@
+(** A theory for checking/proving simulation by symbolic execution.
+
+*)
+
+
+Require Setoid. (* in order to rewrite <-> *)
+Require Export AbstractBasicBlocksDef.
+Require Import List.
+Require Import ImpPrelude.
+Import HConsingDefs.
+
+Module Type PseudoRegDictionary.
+
+Declare Module R: PseudoRegisters.
+
+Parameter t: Type -> Type.
+
+Parameter get: forall {A}, t A -> R.t -> option A.
+
+Parameter set: forall {A}, t A -> R.t -> A -> t A.
+
+Parameter set_spec_eq: forall A d x (v: A),
+  get (set d x v) x = Some v.
+
+Parameter set_spec_diff: forall A d x y (v: A),
+  x <> y -> get (set d x v) y = get d y.
+
+Parameter empty: forall {A}, t A.
+
+Parameter empty_spec: forall A x,
+  get (empty (A:=A)) x = None.
+
+End PseudoRegDictionary.
+
+
+Module SimuTheory (L: SeqLanguage) (Dict: PseudoRegDictionary with Module R:=L.LP.R).
+
+Export L.
+Export LP.
+Export Terms.
+
+(* the symbolic memory:
+  - pre: pre-condition expressing that the computation has not yet abort on a None.
+  - post: the post-condition for each pseudo-register 
+*)
+Record smem:= {pre: genv -> mem -> Prop; post: Dict.t term}.
+
+Coercion post: smem >-> Dict.t.
+
+(** initial symbolic memory *)
+Definition smem_empty := {| pre:=fun _ _ => True; post:=Dict.empty |}.
+
+Definition smem_get (d:Dict.t term) x := 
+   match Dict.get d x with 
+   | None => Input x unknown_hid
+   | Some t => t
+   end.
+
+Fixpoint exp_term (e: exp) (d old: Dict.t term): term :=
+  match e with
+  | PReg x => smem_get d x
+  | Op o le => App o (list_exp_term le d old) unknown_hid
+  | Old e => exp_term e old old
+  end
+with list_exp_term (le: list_exp) (d old: Dict.t term) : list_term :=
+  match le with
+  | Enil => LTnil unknown_hid
+  | Econs e le' => LTcons (exp_term e d old) (list_exp_term le' d old) unknown_hid
+  | LOld le => list_exp_term le old old
+  end.
+
+(** evaluation of the post-condition *)
+Definition smem_eval ge (d: Dict.t term) x (m:mem) :=
+  term_eval ge (smem_get d x) m.
+
+(** assignment of the symbolic memory *)
+Definition smem_set (d:smem) x (t:term) := 
+  {| pre:=(fun ge m => (smem_eval ge d x m) <> None /\ (d.(pre) ge m));
+     post:=Dict.set d x t |}.
+
+Section SIMU_THEORY.
+
+Variable ge: genv.
+
+Lemma set_spec_eq d x t m:
+ smem_eval ge (smem_set d x t) x m = term_eval ge t m.
+Proof.
+  unfold smem_eval, smem_set, smem_get; simpl; rewrite Dict.set_spec_eq; simpl; auto. 
+Qed.
+
+Lemma set_spec_diff d x y t m:
+  x <> y -> smem_eval ge (smem_set d x t) y m = smem_eval ge d y m.
+Proof.
+  intros; unfold smem_eval, smem_set, smem_get; simpl; rewrite Dict.set_spec_diff; simpl; auto. 
+Qed.
+
+Lemma smem_eval_empty x m: smem_eval ge smem_empty x m = Some (m x).
+Proof.
+  unfold smem_eval, smem_get; rewrite Dict.empty_spec; simpl; auto.
+Qed.
+
+Hint Rewrite set_spec_eq smem_eval_empty: dict_rw. 
+
+Fixpoint inst_smem (i: inst) (d old: smem): smem :=
+  match i with
+  | nil => d
+  | (x, e)::i' =>
+     let t:=exp_term e d old in
+     inst_smem i' (smem_set d x t) old
+  end.
+
+Fixpoint bblock_smem_rec (p: bblock) (d: smem): smem :=
+  match p with
+  | nil => d
+  | i::p' =>
+     let d':=inst_smem i d d in
+     bblock_smem_rec p' d'
+  end.
+
+Local Hint Resolve smem_eval_empty.
+
+Definition bblock_smem: bblock -> smem
+ := fun p => bblock_smem_rec p smem_empty.
+
+Lemma inst_smem_pre_monotonic i old: forall d m,
+  (pre (inst_smem i d old) ge m) -> (pre d ge m).
+Proof.
+  induction i as [|[y e] i IHi]; simpl; auto.
+  intros d a H; generalize (IHi _ _ H); clear H IHi.
+  unfold smem_set; simpl; intuition.
+Qed.
+
+Lemma bblock_smem_pre_monotonic p: forall d m,
+  (pre (bblock_smem_rec p d) ge m) -> (pre d ge m).
+Proof.
+  induction p as [|i p' IHp']; simpl; eauto.
+  intros d a H; eapply inst_smem_pre_monotonic; eauto.
+Qed.
+
+Local Hint Resolve inst_smem_pre_monotonic bblock_smem_pre_monotonic.
+
+Lemma term_eval_exp e (od:smem) m0 old:
+  (forall x, smem_eval ge od x m0 = Some (old x)) ->
+  forall d m1,
+   (forall x, smem_eval ge (d:smem) x m0 = Some (m1 x)) ->
+    term_eval ge (exp_term e d od) m0 = exp_eval ge e m1 old.
+Proof.
+  unfold smem_eval in * |- *; intro H.
+  induction e using exp_mut with
+    (P0:=fun l => forall (d:smem) m1, (forall x, term_eval ge (smem_get d x) m0 = Some (m1 x)) -> list_term_eval ge (list_exp_term l d od) m0 = list_exp_eval ge l m1 old);
+  simpl; auto.
+  - intros; erewrite IHe; eauto.
+  - intros. erewrite IHe, IHe0; eauto. 
+Qed.
+
+Lemma inst_smem_abort i m0 x old: forall d,
+    pre (inst_smem i d old) ge m0 ->
+    smem_eval ge d x m0 = None ->
+    smem_eval ge (inst_smem i d old) x m0 = None.
+Proof.
+  induction i as [|[y e] i IHi]; simpl; auto.
+  intros d VALID H; erewrite IHi; eauto. clear IHi.
+  destruct (R.eq_dec x y).
+  * subst; autorewrite with dict_rw.
+    generalize (inst_smem_pre_monotonic _ _ _ _ VALID); clear VALID.
+    unfold smem_set; simpl; intuition congruence.
+  * rewrite set_spec_diff; auto.
+Qed.
+
+Lemma block_smem_rec_abort p m0 x: forall d,
+    pre (bblock_smem_rec p d) ge m0 ->
+    smem_eval ge d x m0 = None ->
+    smem_eval ge (bblock_smem_rec p d) x m0 = None.
+Proof.
+  induction p; simpl; auto.
+  intros d VALID H; erewrite IHp; eauto. clear IHp.
+  eapply inst_smem_abort; eauto.
+Qed.
+
+Lemma inst_smem_Some_correct1 i m0 old (od:smem): 
+  (forall x, smem_eval ge od x m0 = Some (old x)) ->
+  forall (m1 m2: mem) (d: smem), 
+  inst_run ge i m1 old = Some m2 -> 
+  (forall x, smem_eval ge d x m0 = Some (m1 x)) ->
+   forall x, smem_eval ge (inst_smem i d od) x m0 = Some (m2 x).
+Proof.
+  intro X; induction i as [|[x e] i IHi]; simpl; intros m1 m2 d H.
+  - inversion_clear H; eauto.
+  - intros H0 x0.
+    destruct (exp_eval ge e m1 old) eqn:Heqov; try congruence.
+    refine (IHi _ _ _ _ _ _); eauto.
+    clear x0; intros x0.
+    unfold assign; destruct (R.eq_dec x x0).
+    * subst; autorewrite with dict_rw.
+      erewrite term_eval_exp; eauto.
+    * rewrite set_spec_diff; auto.
+Qed.
+
+Lemma bblocks_smem_rec_Some_correct1 p m0: forall (m1 m2: mem) (d: smem), 
+ run ge p m1 = Some m2 -> 
+  (forall x, smem_eval ge d x m0 = Some (m1 x)) ->
+  forall x, smem_eval ge (bblock_smem_rec p d) x m0 = Some (m2 x).
+Proof.
+  Local Hint Resolve inst_smem_Some_correct1.
+  induction p as [ | i p]; simpl; intros m1 m2 d H.
+  - inversion_clear H; eauto.
+  - intros H0 x0.
+    destruct (inst_run ge i m1 m1) eqn: Heqov.
+    + refine (IHp _ _ _ _ _ _); eauto.
+    + inversion H. 
+Qed.
+
+Lemma bblock_smem_Some_correct1 p m0 m1:
+   run ge p m0 = Some m1
+   -> forall x, smem_eval ge (bblock_smem p) x m0 = Some (m1 x).
+Proof.
+  intros; eapply bblocks_smem_rec_Some_correct1; eauto.
+Qed.
+
+Lemma inst_smem_None_correct i m0 old (od: smem):
+   (forall x, smem_eval ge od x m0 = Some (old x)) ->
+  forall m1 d, pre (inst_smem i d od) ge m0 ->
+   (forall x, smem_eval ge d x m0 = Some (m1 x)) ->
+  inst_run ge i m1 old = None -> exists x, smem_eval ge (inst_smem i d od) x m0 = None.
+Proof.
+  intro X; induction i as [|[x e] i IHi]; simpl; intros m1 d.
+  - discriminate.
+  - intros VALID H0.
+    destruct (exp_eval ge e m1 old) eqn: Heqov.
+    + refine (IHi _ _ _ _); eauto.
+      intros x0; unfold assign; destruct (R.eq_dec x x0).
+      * subst; autorewrite with dict_rw. 
+        erewrite term_eval_exp; eauto.
+      * rewrite set_spec_diff; auto.
+    + intuition.
+      constructor 1 with (x:=x); simpl.
+      apply inst_smem_abort; auto.
+      autorewrite with dict_rw.
+      erewrite term_eval_exp; eauto.
+Qed.
+
+Lemma inst_smem_Some_correct2 i m0 old (od: smem):
+  (forall x, smem_eval ge od x m0 = Some (old x)) ->
+  forall (m1 m2: mem) d, 
+  pre (inst_smem i d od) ge m0 ->
+  (forall x, smem_eval ge d x m0 = Some (m1 x)) ->
+  (forall x, smem_eval ge (inst_smem i d od) x m0 = Some (m2 x)) ->
+  res_eq (Some m2) (inst_run ge i m1 old).
+Proof.
+  intro X.
+  induction i as [|[x e] i IHi]; simpl; intros m1 m2 d VALID H0.
+  - intros H; eapply ex_intro; intuition eauto.
+    generalize (H0 x); rewrite H.
+    congruence.
+  - intros H.
+    destruct (exp_eval ge e m1 old) eqn: Heqov.
+    + refine (IHi _ _ _ _ _ _); eauto.
+      intros x0; unfold assign; destruct (R.eq_dec x x0).
+      * subst. autorewrite with dict_rw.
+        erewrite term_eval_exp; eauto.
+      * rewrite set_spec_diff; auto.
+    + generalize (H x).
+      rewrite inst_smem_abort; discriminate || auto.
+      autorewrite with dict_rw. 
+      erewrite term_eval_exp; eauto.
+Qed.
+
+Lemma bblocks_smem_rec_Some_correct2 p m0: forall (m1 m2: mem) d, 
+  pre (bblock_smem_rec p d) ge m0 ->
+  (forall x, smem_eval ge d x m0 = Some (m1 x)) ->
+  (forall x, smem_eval ge (bblock_smem_rec p d) x m0 = Some (m2 x)) ->
+    res_eq (Some m2) (run ge p m1).
+Proof.
+  induction p as [|i p]; simpl; intros m1 m2 d VALID H0.
+  - intros H; eapply ex_intro; intuition eauto.
+    generalize (H0 x); rewrite H.
+    congruence.
+  - intros H.
+     destruct (inst_run ge i m1 m1) eqn: Heqom.
+    + refine (IHp _ _ _ _ _ _); eauto.
+    + assert (X: exists x, term_eval ge (smem_get (inst_smem i d d) x) m0 = None).
+      { eapply inst_smem_None_correct; eauto. }
+      destruct X as [x H1].
+      generalize (H x).
+      erewrite block_smem_rec_abort; eauto.
+      congruence.
+Qed.
+
+
+Lemma bblock_smem_Some_correct2 p m0 m1:
+  pre (bblock_smem p) ge m0 ->
+  (forall x, smem_eval ge (bblock_smem p) x m0 = Some (m1 x))
+  -> res_eq (Some m1) (run ge p m0).
+Proof.
+  intros; eapply bblocks_smem_rec_Some_correct2; eauto.
+Qed.
+
+Lemma inst_valid i m0 old (od:smem):
+  (forall x, smem_eval ge od x m0 = Some (old x)) ->
+  forall (m1 m2: mem) (d: smem), 
+  pre d ge m0 ->
+  inst_run ge i m1 old = Some m2 ->
+  (forall x, smem_eval ge d x m0 = Some (m1 x)) ->
+   pre (inst_smem i d od) ge m0.
+Proof.
+  induction i as [|[x e] i IHi]; simpl; auto.
+  intros Hold m1 m2 d VALID0 H Hm1.
+  destruct (exp_eval ge e m1 old) eqn: Heq; simpl; try congruence.
+  eapply IHi; eauto.
+  + unfold smem_set in * |- *; simpl. 
+    rewrite Hm1; intuition congruence.
+  + intros x0. unfold assign; destruct (R.eq_dec x x0).
+    * subst; autorewrite with dict_rw.
+      erewrite term_eval_exp; eauto.
+    * rewrite set_spec_diff; auto.
+Qed.
+
+
+Lemma block_smem_rec_valid p m0: forall (m1 m2: mem) (d:smem), 
+  pre d ge m0 ->
+  run ge p m1 = Some m2 -> 
+  (forall x, smem_eval ge d x m0 = Some (m1 x)) ->
+  pre (bblock_smem_rec p d) ge m0.
+Proof.
+  Local Hint Resolve inst_valid.
+  induction p as [ | i p]; simpl; intros m1 d H; auto.
+  intros H0 H1.
+  destruct (inst_run ge i m1 m1) eqn: Heqov; eauto.
+  congruence.
+Qed.
+
+Lemma bblock_smem_valid p m0 m1:
+  run ge p m0 = Some m1 ->
+  pre (bblock_smem p) ge m0.
+Proof.
+  intros; eapply block_smem_rec_valid; eauto.
+  unfold smem_empty; simpl. auto.
+Qed.
+
+Definition svalid ge d m := pre d ge m /\ forall x, smem_eval ge d x m <> None.
+
+Theorem bblock_smem_simu p1 p2:
+  (forall m, svalid ge (bblock_smem p1) m -> svalid ge (bblock_smem p2) m) ->
+  (forall m0 x m1, svalid ge (bblock_smem p1) m0 -> smem_eval ge (bblock_smem p1) x m0 = Some m1 ->
+                   smem_eval ge (bblock_smem p2) x m0 = Some m1) ->
+   bblock_simu ge p1 p2.
+Proof.
+  Local Hint Resolve bblock_smem_valid bblock_smem_Some_correct1.
+  unfold svalid; intros INCL EQUIV m DONTFAIL.
+  destruct (run ge p1 m) as [m1|] eqn: RUN1; simpl; try congruence.
+  assert (X: forall x, smem_eval ge (bblock_smem p1) x m = Some (m1 x)); eauto.
+  eapply bblock_smem_Some_correct2; eauto.
+  + destruct (INCL m); intuition eauto.
+    congruence.
+  + intro x; apply EQUIV; intuition eauto.
+    congruence.
+Qed.
+
+Lemma svalid_set_decompose_1 d t x m:
+  svalid ge (smem_set d x t) m -> svalid ge d m.
+Proof.
+  unfold svalid; intros ((PRE1 & PRE2) & VALID); split.
+  + intuition.
+  + intros x0 H. case (R.eq_dec x x0).
+    * intuition congruence.
+    * intros DIFF; eapply VALID. erewrite set_spec_diff; eauto.
+Qed.
+
+Lemma svalid_set_decompose_2 d t x m:
+  svalid ge (smem_set d x t) m -> term_eval ge t m <> None.
+Proof.
+  unfold svalid; intros ((PRE1 & PRE2) & VALID) H.
+  generalize (VALID x); autorewrite with dict_rw.
+  tauto.
+Qed.
+
+Lemma svalid_set_proof d x t m:
+  svalid ge d m -> term_eval ge t m <> None -> svalid ge (smem_set d x t) m.
+Proof.
+  unfold svalid; intros (PRE & VALID) PREt. split.
+  + split; auto.
+  + intros x0; case (R.eq_dec x x0).
+    - intros; subst; autorewrite with dict_rw. auto.
+    - intros. rewrite set_spec_diff; auto. 
+Qed.
+
+End SIMU_THEORY.
+
+End SimuTheory.
+
+Require Import PArith.
+Require Import FMapPositive.
+
+Module PosDict <: PseudoRegDictionary with Module R:=Pos.
+
+Module R:=Pos.
+
+Definition t:=PositiveMap.t.
+
+Definition get {A} (d:t A) (x:R.t): option A 
+ := PositiveMap.find x d.
+
+Definition set {A} (d:t A) (x:R.t) (v:A): t A
+ := PositiveMap.add x v d.
+
+Local Hint Unfold PositiveMap.E.eq.
+
+Lemma set_spec_eq A d x (v: A):
+  get (set d x v) x = Some v.
+Proof.
+  unfold get, set; apply PositiveMap.add_1; auto.
+Qed.
+
+Lemma set_spec_diff A d x y (v: A):
+  x <> y -> get (set d x v) y = get d y.
+Proof.
+  unfold get, set; intros; apply PositiveMap.gso; auto.
+Qed.
+
+Definition empty {A}: t A := PositiveMap.empty A.
+
+Lemma empty_spec A x:
+  get (empty (A:=A)) x = None.
+Proof.
+  unfold get, empty; apply PositiveMap.gempty; auto.
+Qed.
+
+End PosDict.
